Mutual Attestation Adequacy

theories/examples/enclaves/mutual_attestation_adequacy.v
@@ -4,16 +4,15 @@ From cap_machine Require Import proofmode.
 From cap_machine Require Import assert macros_new.
 From cap_machine Require Import attestation_adequacy_template.
 From cap_machine Require Import
-  trusted_compute_code
-  trusted_compute_enclave_spec
-  trusted_compute_spec
+  mutual_attestation_code
+  mutual_attestation_spec
 .
 
 Class memory_layout `{MachineParameters} := {
   (* Verifier code *)
   verifier_start : Addr;
   verifier_end : Addr;
-  verifier_size: (verifier_start + trusted_compute_main_len = Some verifier_end)%a;
+  verifier_size: (verifier_start + mutual_attestation_main_len = Some verifier_end)%a;
   verifier_region: list Addr;
   verifier_region_correct:
     verifier_region = (finz.seq_between verifier_start verifier_end);
@@ -53,10 +52,15 @@ Class memory_layout `{MachineParameters} := {
   link_table_region_correct:
     link_table_region = (finz.seq_between l_assert_start l_assert_end);
 
-  (* TC enclave *)
-  tc_enclave_start : Addr;
-  tc_enclave_end : Addr;
-  tc_enclave_size : (tc_enclave_start + (trusted_compute_enclave_code_len + 1))%a =  Some tc_enclave_end;
+  (* MA enclave A *)
+  ma_enclave_A_start : Addr;
+  ma_enclave_A_end : Addr;
+  ma_enclave_A_size : (ma_enclave_A_start + (mutual_attest_enclave_A_code_len + 1))%a =  Some ma_enclave_A_end;
+
+  (* MA enclave B *)
+  ma_enclave_B_start : Addr;
+  ma_enclave_B_end : Addr;
+  ma_enclave_B_size : (ma_enclave_B_start + (mutual_attest_enclave_B_code_len + 1))%a =  Some ma_enclave_B_end;
 
   regions_disjoints :
   verifier_region ## adv_region ∧
@@ -67,21 +71,21 @@ Class memory_layout `{MachineParameters} := {
   l_assert_region ## link_table_region;
 }.
 
-Local Instance trusted_compute_concrete `{memory_layout} : TrustedCompute.
-Proof. apply (Build_TrustedCompute tc_enclave_start). Defined.
+Local Instance mutual_attest_concrete `{memory_layout} : MutualAttestation.
+Proof. apply (Build_MutualAttestation ma_enclave_A_start ma_enclave_B_start). Defined.
 
 Definition link_tbl_cap `{memory_layout} :=
  WCap RO link_table_start link_table_end link_table_start.
 
-Program Definition tc_verifier_prog `{memory_layout} : prog :=
+Program Definition ma_verifier_prog `{memory_layout} : prog :=
   let link_cap := link_tbl_cap in
-  let a_data := (verifier_start ^+ trusted_compute_main_code_len)%a in
+  let a_data := (verifier_start ^+ mutual_attestation_main_code_len)%a in
   let data_cap := WCap RWX verifier_start verifier_end a_data  in
   {| prog_start := verifier_start ;
      prog_end := verifier_end ;
      prog_instrs :=
-      (lword_get_word <$> (trusted_compute_main_code 0))
-       ++ [link_cap ; data_cap];
+      (lword_get_word <$> (mutual_attestation_main_code 0))
+       ++ [link_cap];
      prog_size := _ |}.
 Next Obligation.
   intros MP ML *.
@@ -117,7 +121,7 @@ Definition tbl_assert_tbl `{memory_layout} : assert_tbl :=
     tbl_size := link_table_size;
   |}.
 
-Section tc_adequacy.
+Section ma_adequacy.
   Context {Σ:gFunctors}
           `{MP: MachineParameters}
           {ceriseg:ceriseG Σ} {sealsg: sealStoreG Σ}
@@ -125,12 +129,12 @@ Section tc_adequacy.
           {memlayout: memory_layout}
   .
 
-  Definition trusted_computeN : namespace := nroot .@ "trusted_compute".
-  Definition link_tableN := (trusted_computeN.@"link_table").
-  Definition tc_mainN := (trusted_computeN.@"main").
-  Lemma tc_correct :
+  Definition mutual_attestN := (nroot.@"mutual_attest").
+  Definition link_tableN := (mutual_attestN.@"link_table").
+  Definition ma_mainN := (mutual_attestN.@"main").
+  Lemma ma_correct :
     let vinit := 0%nat in
-    let P := tc_verifier_prog in
+    let P := ma_verifier_prog in
     let Adv := adv_prog in
     let AssertLib := assert_layout in
     let RA := reserved_addresses_assert AssertLib vinit in
@@ -168,7 +172,7 @@ Section tc_adequacy.
       "(#Hinv & #Hassert & Hown & HPC & Hr_adv & Hrmap & Hprog & Hadv & Hlink & HEC & Hseal_store)".
 
     simpl.
-    iMod ( custom_enclaves_inv_alloc (enclaves_map := contract_tc_enclaves_map) with
+    iMod ( custom_enclaves_inv_alloc (enclaves_map := contract_ma_enclaves_map) with
            "[$HEC $Hseal_store]") as "#Hsystem_inv".
 
     iMod (na_inv_alloc logrel_nais ⊤ link_tableN
@@ -220,23 +224,19 @@ Section tc_adequacy.
             rewrite finz_seq_between_length /finz.dist /=. solve_addr+Hadv_size'.
     }
 
-    set (a_data := (prog_start P ^+ length (trusted_compute_main_code 0))%a).
+    set (a_data := (prog_start P ^+ length (mutual_attestation_main_code 0))%a).
     set (link_cap := word_to_lword link_tbl_cap vinit).
-    iMod (na_inv_alloc logrel_nais ⊤ tc_mainN
-           (codefrag (prog_start P) vinit (trusted_compute_main_code 0)
-            ∗ (a_data, vinit) ↦ₐ link_cap
-            ∗ ((a_data ^+ 1)%a, vinit) ↦ₐ LCap RWX (prog_start P) (prog_end P) a_data vinit)
+    iMod (na_inv_alloc logrel_nais ⊤ ma_mainN
+           (codefrag (prog_start P) vinit (mutual_attestation_main_code 0) ∗ (a_data, vinit) ↦ₐ link_cap)
          with "[Hprog]") as "#Hprog".
     { iNext.
       replace (prog_region P)
         with
         (mkregion verifier_start verifier_end
-                 ((lword_get_word <$> trusted_compute_main_code 0) ++
-                 [link_tbl_cap;
-                  WCap RWX verifier_start verifier_end (verifier_start ^+ trusted_compute_main_code_len)%a])
+                 ((lword_get_word <$> mutual_attestation_main_code 0) ++ [link_tbl_cap])
               ) by done.
       pose proof verifier_size as Hsize_verifier.
-      rewrite /trusted_compute_main_len in Hsize_verifier.
+      rewrite /mutual_attestation_main_len in Hsize_verifier.
       rewrite mkregion_app; last done.
       rewrite memory_to_lmemory_union.
       iDestruct (big_sepM_union with "Hprog") as "[Hprog Hdata]".
@@ -246,8 +246,7 @@ Section tc_adequacy.
         + rewrite fmap_length.
           rewrite finz_seq_between_length.
           apply finz_dist_add.
-          exists (verifier_start ^+ length (trusted_compute_main_code 0))%a.
-          cbn in *.
+          exists (verifier_start ^+ length (mutual_attestation_main_code 0))%a.
           solve_addr.
         + apply Forall_forall.
           intros a Ha.
@@ -258,42 +257,12 @@ Section tc_adequacy.
             solve_addr.
           * rewrite fmap_length.
             rewrite finz_seq_between_length.
-            cbn.
-            rewrite finz_dist_S; last solve_addr.
             rewrite finz_dist_S; last solve_addr.
             rewrite finz_dist_0; last solve_addr.
             done.
       }
 
-      replace ([link_tbl_cap; WCap RWX verifier_start verifier_end (verifier_start ^+ trusted_compute_main_code_len)%a])
-        with ([link_tbl_cap]++[WCap RWX verifier_start verifier_end
-                                 (verifier_start ^+ trusted_compute_main_code_len)%a]); last by cbn.
-      rewrite mkregion_app; last solve_addr.
-      rewrite memory_to_lmemory_union.
-      iDestruct (big_sepM_union with "Hdata") as "[Hdata1 Hdata2]".
-      { apply memory_to_lmemory_disjoint.
-        rewrite /mkregion.
-        apply map_disjoint_list_to_map_zip_l.
-        + rewrite finz_seq_between_length.
-          apply finz_dist_add.
-          exists (verifier_start ^+ 38)%a.
-          cbn in *.
-          solve_addr.
-        + apply Forall_forall.
-          intros a Ha.
-          apply not_elem_of_list_to_map.
-          rewrite fst_zip.
-          * rewrite elem_of_finz_seq_between in Ha.
-            rewrite not_elem_of_finz_seq_between.
-            solve_addr.
-          * rewrite finz_seq_between_length.
-            cbn.
-            rewrite finz_dist_S; last solve_addr.
-            rewrite finz_dist_0; last solve_addr.
-            done.
-      }
-
-      iSplitL "Hprog"; [|iSplitL "Hdata1"].
+      iSplitL "Hprog".
       - rewrite /codefrag /region_mapsto.
         iApply (big_sepM_to_big_sepL2 with "[Hprog]").
         { apply NoDup_fmap; first (intros ? ? ?; by simplify_eq).
@@ -303,23 +272,19 @@ Section tc_adequacy.
           rewrite finz_seq_between_length.
           cbn.
           apply finz_dist_add.
-          exists (verifier_start ^+ 37%nat)%a.
+          exists (verifier_start ^+ 72%nat)%a.
           solve_addr.
         }
         iEval (rewrite memory_to_lmemory_mk_logical_region_map) in "Hprog".
         iFrame.
-      - iEval (rewrite memory_to_lmemory_mk_logical_region_map) in "Hdata1".
+      - iEval (rewrite memory_to_lmemory_mk_logical_region_map) in "Hdata".
         rewrite finz_seq_between_cons; last solve_addr.
         rewrite finz_seq_between_empty; last solve_addr.
-        iDestruct (big_sepM_insert_delete with "Hdata1") as "[$ _]".
-      - iEval (rewrite memory_to_lmemory_mk_logical_region_map) in "Hdata2".
-        rewrite finz_seq_between_cons; last solve_addr.
-        rewrite finz_seq_between_empty; last solve_addr.
-        iDestruct (big_sepM_insert_delete with "Hdata2") as "[$ _]".
+        iDestruct (big_sepM_insert_delete with "Hdata") as "[$ _]".
     }
 
-    iAssert (tc_main_inv verifier_start verifier_end vinit (trusted_compute_main_code 0) a_data
-               link_cap tc_mainN) with "Hprog" as "#Hprog_inv".
+    iAssert (ma_main_inv verifier_start vinit (mutual_attestation_main_code 0) a_data
+               link_cap ma_mainN) with "Hprog" as "#Hprog_inv".
     iAssert (assert_inv (assert_start AssertLib) (assert_flag AssertLib) (assert_end AssertLib)
                vinit assertN)
       with "Hassert" as "Hassert_inv".
@@ -347,21 +312,22 @@ Section tc_adequacy.
     }
 
     pose proof ( verifier_size ) as Hverifier_size.
-    replace verifier_end with (verifier_start ^+ trusted_compute_main_len)%a by solve_addr.
+    replace verifier_end with (verifier_start ^+ mutual_attestation_main_len)%a by solve_addr.
 
     iApply (wp_wand with "[-]").
-    - iApply (trusted_compute_full_run_spec with
-      "[$Hadv $Hsystem_inv $Hinv_link $Hassert $Hprog_inv $Hflag_inv ] [ $HPC $Hown $Hr_adv $Hrmap]"); auto.
+    - subst a_data link_cap.
+      iApply (mutual_attest_full_run_spec with
+      "[$Hadv $Hsystem_inv $Hinv_link $Hassert $Hprog_inv $Hflag_inv ] [ $HPC $Hown $Hr_adv $Hrmap]").
       + solve_ndisj.
       + solve_ndisj.
       + solve_ndisj.
-      + subst P; rewrite /tc_verifier_prog /=.
+      + subst P; rewrite /ma_verifier_prog /=.
         solve_addr.
       + rewrite /SubBounds.
         split; first solve_addr.
         split; last solve_addr.
-        subst P; rewrite /tc_verifier_prog /=.
-        rewrite /trusted_compute_main_len.
+        subst P; rewrite /ma_verifier_prog /=.
+        rewrite /mutual_attestation_main_len.
         solve_addr.
       + pose proof link_table_size.
         cbn; solve_addr.
@@ -373,15 +339,15 @@ Section tc_adequacy.
     - by iIntros (v) "H".
   Qed.
 
-End tc_adequacy.
+End ma_adequacy.
 
 
-Theorem tc_enclaves_adequacy `{memory_layout}
+Theorem ma_enclaves_adequacy `{memory_layout}
     (m m': Mem) (reg reg': Reg) (etbl' : ETable) (ecur' : ENum)
     (es: list cap_lang.expr):
-  is_initial_memory tc_verifier_prog adv_prog assert_layout tbl_assert_tbl m →
+  is_initial_memory ma_verifier_prog adv_prog assert_layout tbl_assert_tbl m →
   is_complete_memory m →
-  is_initial_registers tc_verifier_prog adv_prog assert_layout tbl_assert_tbl reg r_t0 →
+  is_initial_registers ma_verifier_prog adv_prog assert_layout tbl_assert_tbl reg r_t0 →
   is_complete_registers reg m →
   Forall (λ w, is_z w = true \/ in_region w adv_start adv_end) (prog_instrs adv_prog) →
 
@@ -391,12 +357,12 @@ Theorem tc_enclaves_adequacy `{memory_layout}
 Proof.
   intros ? ? ? ? Hints.
   set (Σ' := #[]).
-  pose proof (template_adequacy Σ' tc_verifier_prog adv_prog assert_layout tbl_assert_tbl) as Hadequacy.
+  pose proof (template_adequacy Σ' ma_verifier_prog adv_prog assert_layout tbl_assert_tbl) as Hadequacy.
   eapply Hadequacy;eauto.
   - eapply adequacy_flag_inv_is_initial_memory; eauto.
   - intros Σ ? ? ? ? ? ?.
     iIntros "(?&?&?&?&?&?&?&?&?&?&?)".
-    iApply tc_correct; eauto; last iFrame.
+    iApply ma_correct; eauto; last iFrame.
 
     cbn.
     clear.
